add type_alive

examples/tagged_ptr.c
@@ -10,39 +10,36 @@ typedef unsigned char tag_t;
 
 //@rc::inlined Notation TAG_MOD := (8%nat) (only parsing).
 
-[[rc::parameters("r: {loc * Z}", "ty: type", "v: val", "P: {iProp Σ}")]]
+[[rc::parameters("r: {loc * Z}", "ty: type", "v: val")]]
 [[rc::args("at_value<v, r @ &tagged<TAG_MOD, ty>>")]]
-[[rc::requires("{AllocAlive ty Own P}", "[P]")]]
+[[rc::requires("[type_alive_own ty]")]]
 [[rc::returns("{r.2} @ int<u8>")]]
-[[rc::ensures("v : r @ &tagged<TAG_MOD, ty>", "{0 ≤ r.2 < TAG_MOD}", "[P]")]]
+[[rc::ensures("v : r @ &tagged<TAG_MOD, ty>", "{0 ≤ r.2 < TAG_MOD}")]]
 tag_t tag_of(void* p){
   return ((uintptr_t) p) % TAG_MOD;
 }
 
-[[rc::parameters("r: {loc * Z}", "t: Z", "ty: type", "P: {iProp Σ}")]]
+[[rc::parameters("r: {loc * Z}", "t: Z", "ty: type")]]
 [[rc::args("r @ &tagged<TAG_MOD, ty>", "t @ int<u8>")]]
-[[rc::requires("{0 ≤ t < TAG_MOD}", "{AllocAlive ty Own P}", "[P]")]]
+[[rc::requires("{0 ≤ t < TAG_MOD}", "[type_alive_own ty]")]]
 [[rc::returns("{(r.1, t)} @ &tagged<TAG_MOD, ty>")]]
-[[rc::ensures("[P]")]]
 void* tag(void* p, tag_t t){
   tag_t old_t = tag_of(p);
   return rc_copy_alloc_id((uintptr_t) p - old_t + t, p);
 }
 
-[[rc::parameters("r: {loc * Z}", "ty: type", "P: {iProp Σ}")]]
+[[rc::parameters("r: {loc * Z}", "ty: type")]]
 [[rc::args("r @ &tagged<TAG_MOD, ty>")]]
-[[rc::requires("{AllocAlive ty Own P}", "[P]")]]
+[[rc::requires("[type_alive_own ty]")]]
 [[rc::returns("{r.1} @ &own<ty>")]]
-[[rc::ensures("[P]")]]
 void* untag(void* p){
   return tag(p, 0);
 }
 
-[[rc::parameters("r: {loc * Z}", "ty: type", "P: {iProp Σ}")]]
+[[rc::parameters("r: {loc * Z}", "ty: type")]]
 [[rc::args("r @ &tagged<TAG_MOD, ty>")]]
-[[rc::requires("{AllocAlive ty Own P}", "[P]")]]
+[[rc::requires("[type_alive_own ty]")]]
 [[rc::returns("{r.1} @ &own<ty>")]]
-[[rc::ensures("[P]")]]
 void* untag2(void* p){
   uintptr_t i = (uintptr_t) p;
   return rc_copy_alloc_id(i - i % TAG_MOD, p);
