examples/proofs/tagged_ptr/generated_proof_tag.v
@@ -13,7 +13,7 @@ Section proof_tag.
     typed_function (impl_tag global_tag_of) type_of_tag.
   Proof.
     Open Scope printing_sugar.
-    start_function "tag" ([[[r t] ty] P]) => arg_p arg_t local_old_t.
+    start_function "tag" ([[r t] ty]) => arg_p arg_t local_old_t.
     split_blocks ((
       ∅
     )%I : gmap label (iProp Σ)) ((
